Core/Examples/Boolean.lean
@@ -19,7 +19,9 @@ not = λ x → case x of
                _ → False
 -/
 def notTerm : Term := λ[ .closed , .global "Bool" ]
-  match! #0 v[
+  match! #0
+         v[ "True", "False" ]
+         v[
          g# "False",
          g# "True" ]
 
@@ -33,9 +35,9 @@ def notTerm : Term := λ[ .closed , .global "Bool" ]
                        False → True
  -/
 def eqBool : Term := λ[ .closed,  .global "Bool" ] λ[ .closed, .global "Bool" ]
-  match! #1
-   v[ match! #0 v[ g#"True", g#"False"] ,
-      match! #0 v[ g# "False", g# "False"]
+  match! #1 v[ "True", "False" ]
+   v[ match! #0 v[ "True", "False" ] v[ g#"True", g#"False"] ,
+      match! #0 v[ "True", "False" ] v[ g# "False", g# "False"]
     ]
 
 
@@ -67,24 +69,30 @@ def t2 : Term := (g#"eq" •[ gt#"Bool" ]  • (g#"EqBool" •[  gt#"Bool" ] •
 #eval! eval_loop EqBoolCtx t1
 #eval! eval_loop EqBoolCtx t2
 
--- #eval! eval EqBoolCtx t1
--- def t3 := Option.getD (eval EqBoolCtx t1) `0
--- #eval! eval EqBoolCtx t3
--- def t4 := Option.getD (eval EqBoolCtx t3) `0
--- #eval! eval EqBoolCtx t4
--- def t5 := Option.getD (eval EqBoolCtx t4) `0
--- #eval! eval EqBoolCtx t5
--- def t6 := Option.getD (eval EqBoolCtx t5) `0
--- #eval! eval EqBoolCtx t6
--- def t7 := Option.getD (eval EqBoolCtx t6) `0
--- #eval! eval EqBoolCtx t7
--- def t8 := Option.getD (eval EqBoolCtx t7) `0
--- #eval! eval EqBoolCtx t8
--- def t9 := Option.getD (eval EqBoolCtx t8) `0
--- #eval! eval EqBoolCtx t9
--- def t10 := Option.getD (eval EqBoolCtx t9) `0
--- #eval! eval EqBoolCtx t10
--- def t11 := Option.getD (eval EqBoolCtx t10) `0
--- #eval! eval EqBoolCtx t11
--- def t12 := Option.getD (eval EqBoolCtx t11) `0
--- #eval! eval EqBoolCtx t12
+#eval! eval EqBoolCtx t1
+def t3 := Option.getD (eval EqBoolCtx t1) `0
+#eval! eval EqBoolCtx t3
+def t4 := Option.getD (eval EqBoolCtx t3) `0
+#eval! eval EqBoolCtx t4
+def t5 := Option.getD (eval EqBoolCtx t4) `0
+#eval! eval EqBoolCtx t5
+def t6 := Option.getD (eval EqBoolCtx t5) `0
+#eval! eval EqBoolCtx t6
+def t7 := Option.getD (eval EqBoolCtx t6) `0
+#eval! eval EqBoolCtx t7
+def t8 := Option.getD (eval EqBoolCtx t7) `0
+#eval! eval EqBoolCtx t8
+def t9 := Option.getD (eval EqBoolCtx t8) `0
+#eval! eval EqBoolCtx t9
+def t10 := Option.getD (eval EqBoolCtx t9) `0
+#eval! eval EqBoolCtx t10
+def t11 := Option.getD (eval EqBoolCtx t10) `0
+#eval! eval EqBoolCtx t11
+def t12 := Option.getD (eval EqBoolCtx t11) `0
+#eval! eval EqBoolCtx t12
+def t13 := Option.getD (eval EqBoolCtx t12) `0
+#eval! eval EqBoolCtx t13
+def t14 := Option.getD (eval EqBoolCtx t13) `0
+#eval! eval EqBoolCtx t14
+def t15 := Option.getD (eval EqBoolCtx t14) `0
+#eval! eval EqBoolCtx t15
