Core/Ty/Structure.lean
@@ -14,3 +14,28 @@ def Ty.arity : Ty -> Nat
 | arrow _ _ B => B.arity + 1
 | ∀[_] P => P.arity + 1
 | _ => 0
+
+
+inductive TyTeleElem
+| kind (k  : Kind)
+| ty (b : BaseKind) (t : Ty)
+
+def TyTele  := List TyTeleElem
+
+def Ty.split : Ty -> TyTele × Ty
+| .arrow K A B =>
+  let (tys, b) := B.split
+  (.ty K A :: tys, b)
+| .all K B =>
+  let (tys, b) := B.split
+  (.kind K :: tys, b)
+| t => ([], t)
+
+def Ty.mk_from_tele : TyTele -> Ty -> Ty
+| .nil , t => t
+| .cons (.ty K A) tys, t =>
+  let r := t.mk_from_tele tys
+  A -[K]> r
+| .cons (.kind K) tys, t =>
+  let r := t.mk_from_tele tys
+  ∀[K] r
